---
layout: default
title: Algebraic Identities
---

<div>
  <h2>Algebraic Identities</h2>

  <hr>

  <h3>1. Common Algebraic Identities</h3>
  <ul>
    <li>\((a + b)^2 = a^2 + 2ab + b^2\)</li>
    <li>\((a - b)^2 = a^2 - 2ab + b^2\)</li>
    <li>\((a + b)(a - b) = a^2 - b^2\)</li>
  </ul>

  <p><strong>Example:</strong> Expand \((x + 5)^2\):</p>
  <div>$$
  (x + 5)^2 = x^2 + 2(5)(x) + 5^2 = x^2 + 10x + 25
  $$</div>

  <hr>

  <h3>2. Completing the Square</h3>
  <p>This rewrites a quadratic in the form \(x^2 + bx + c\) as \((x + p)^2 + q\).</p>
  <p><strong>Steps:</strong></p>
  <ul>
    <li>Take half of \(b\) and square it</li>
    <li>Add and subtract that square inside the expression</li>
    <li>Factor and simplify</li>
  </ul>

  <p><strong>Example:</strong> Complete the square for \(x^2 + 6x + 2\):</p>
  <div>Take half of 6: \(3\), square it: \(9\)</div>
  <div>$$
  x^2 + 6x + 2 = (x^2 + 6x + 9) - 9 + 2 = (x + 3)^2 - 7
  $$</div>

  <hr>

  <h3>3. Changing the Subject of a Formula</h3>
  <p>To change the subject, isolate the desired variable on one side using inverse operations.</p>

  <p><strong>Example:</strong> Make \(x\) the subject in \(y = 3x + 5\)</p>
  <div>Subtract 5 from both sides:</div>
  <div>$$
  y - 5 = 3x
  $$</div>
  <div>Now divide both sides by 3:</div>
  <div>$$
  x = \frac{y - 5}{3}
  $$</div>

  <hr>

  <h3>4. Irrational Equations (Square Roots)</h3>
  <p>These involve square roots. The usual method is to isolate the root and then square both sides to eliminate it.</p>

  <p><strong>Example:</strong> Solve \(\sqrt{x + 3} = 5\)</p>
  <div>Square both sides:</div>
  <div>$$
  (\sqrt{x + 3})^2 = 5^2 \Rightarrow x + 3 = 25
  $$</div>
  <div>Subtract 3:</div>
  <div>$$
  x = 22
  $$</div>

  <p><strong>Important:</strong> Always check your answer in the original equation to avoid extraneous solutions.</p>

</div>
