---
layout: default
title: Simultaneous Equations
---

<div>
  <h2>Simultaneous Equations</h2>

  <p>Simultaneous equations are two or more equations that are solved together because they share the same variables. The solution is the point(s) where the equations are all true at the same time.</p>

  <hr>

  <h3>1. Line and Line (Two Linear Equations)</h3>
  <p>This involves solving two equations that each represent a straight line. The solution is the point where the two lines intersect.</p>

  <p><strong>Example:</strong> Solve the system:</p>
  <div>
  \( \text{Equation 1: } x + y = 7 \)  
  <br>
  \( \text{Equation 2: } x - y = 3 \)
  </div>

  <p><strong>Step 1:</strong> Add the equations:</p>
  <div>$$
  (x + y) + (x - y) = 7 + 3 \Rightarrow 2x = 10 \Rightarrow x = 5
  $$</div>

  <p><strong>Step 2:</strong> Substitute into one of the original equations:</p>
  <div>$$
  x + y = 7 \Rightarrow 5 + y = 7 \Rightarrow y = 2
  $$</div>

  <p><strong>Solution:</strong> \(x = 5, y = 2\)</p>

  <hr>

  <h3>2. Line and Curve (Linear and Quadratic)</h3>
  <p>This involves solving a straight-line equation and a quadratic equation. The solution(s) are the points where the line intersects the curve.</p>

  <p><strong>Example:</strong> Solve:</p>
  <div>
  \( \text{Equation 1: } y = x + 1 \)  
  <br>
  \( \text{Equation 2: } y = x^2 \)
  </div>

  <p><strong>Step 1:</strong> Since both equal \(y\), set the equations equal to each other:</p>
  <div>$$
  x + 1 = x^2
  $$</div>
  <div>Rearrange: \(x^2 - x - 1 = 0\)</div>

  <p><strong>Step 2:</strong> Solve using the quadratic formula:</p>
  <div>$$
  x = \frac{1 \pm \sqrt{1^2 + 4(1)(1)}}{2} = \frac{1 \pm \sqrt{5}}{2}
  $$</div>

  <p><strong>Step 3:</strong> Substitute back into \(y = x + 1\) to find \(y\)</p>
  <p>There are two solutions — one for each \(x\)-value.</p>

  <hr>

  <h3>3. Simultaneous Equations in Three Unknowns</h3>
  <p>This involves solving three equations with three variables (usually \(x\), \(y\), and \(z\)). The solution is the point where all three equations meet in space.</p>

  <p><strong>Example:</strong> Solve:</p>
  <div>
  \(x + y + z = 6\)  
  <br>
  \(2x - y + z = 3\)  
  <br>
  \(x + 2y - z = 4\)
  </div>

  <p><strong>Step 1:</strong> Eliminate one variable using two pairs of equations. Let’s eliminate \(z\):</p>

  <p>Add Equation 1 and Equation 2:</p>
  <div>$$
  (x + y + z) + (2x - y + z) = 6 + 3 \Rightarrow 3x + 2z = 9 \quad \text{(Equation A)}
  $$</div>

  <p>Add Equation 1 and Equation 3:</p>
  <div>$$
  (x + y + z) + (x + 2y - z) = 6 + 4 \Rightarrow 2x + 3y = 10 \quad \text{(Equation B)}
  $$</div>

  <p><strong>Step 2:</strong> Solve Equations A and B using substitution or elimination (continue process...)</p>
  <p><strong>Final Answer:</strong> After solving, you’ll get one value for each of \(x\), \(y\), and \(z\).</p>

  <p>Note: These steps can be long — they are often solved using substitution, elimination, or matrices on a calculator.</p>

</div>
