---
layout: default
title: Surds
---

<div>
  <h2>Surds</h2>

  <hr>

  <h3>1. What is a Surd?</h3>
  <p>A surd is an irrational number that cannot be simplified to remove the square root (or cube root, etc.). For example, \(\sqrt{2}\), \(\sqrt{3}\), and \(\sqrt{5}\) are surds.</p>
  <p>\(\sqrt{4} = 2\) is not a surd because the square root is a whole number.</p>

  <hr>

  <h3>2. Properties of Surds</h3>
  <ul>
    <li>\(\sqrt{a} \times \sqrt{b} = \sqrt{ab}\)</li>
    <li>\(\frac{\sqrt{a}}{\sqrt{b}} = \sqrt{\frac{a}{b}}\)</li>
    <li>\((\sqrt{a})^2 = a\)</li>
  </ul>

  <p><strong>Example 1:</strong> \(\sqrt{3} \times \sqrt{12} = \sqrt{36} = 6\)</p>
  <p><strong>Example 2:</strong> \(\frac{\sqrt{8}}{\sqrt{2}} = \sqrt{\frac{8}{2}} = \sqrt{4} = 2\)</p>
  <p><strong>Example 3:</strong> \((\sqrt{7})^2 = 7\)</p>

  <hr>

  <h3>3. The Conjugate of a Surd</h3>
  <p>The conjugate of an expression like \(a + \sqrt{b}\) is \(a - \sqrt{b}\), and vice versa.</p>
  <p>Multiplying by the conjugate removes the surd from a binomial expression using the identity \((a + b)(a - b) = a^2 - b^2\).</p>

  <p><strong>Example:</strong> Multiply \((3 + \sqrt{5})(3 - \sqrt{5})\):</p>
  <div>$$
  (3 + \sqrt{5})(3 - \sqrt{5}) = 3^2 - (\sqrt{5})^2 = 9 - 5 = 4
  $$</div>

  <hr>

  <h3>4. Rationalising the Denominator</h3>
  <p>To rationalise the denominator means to eliminate any surd from the bottom (denominator) of a fraction.</p>

  <p><strong>Case 1:</strong> If the denominator is a single surd:</p>
  <p><strong>Example:</strong> \(\frac{1}{\sqrt{2}}\)</p>
  <p>Multiply top and bottom by \(\sqrt{2}\):</p>
  <div>$$
  \frac{1}{\sqrt{2}} \times \frac{\sqrt{2}}{\sqrt{2}} = \frac{\sqrt{2}}{2}
  $$</div>

  <p><strong>Case 2:</strong> If the denominator is a binomial with a surd:</p>
  <p><strong>Example:</strong> \(\frac{1}{3 + \sqrt{2}}\)</p>
  <p>Multiply top and bottom by the conjugate \(3 - \sqrt{2}\):</p>
  <div>$$
  \frac{1}{3 + \sqrt{2}} \times \frac{3 - \sqrt{2}}{3 - \sqrt{2}} = \frac{3 - \sqrt{2}}{(3 + \sqrt{2})(3 - \sqrt{2})}
  $$</div>
  <div>Now simplify the denominator:</div>
  <div>$$
  (3 + \sqrt{2})(3 - \sqrt{2}) = 9 - 2 = 7
  $$</div>
  <div>So the final answer is:</div>
  <div>$$
  \frac{3 - \sqrt{2}}{7}
  $$</div>

</div>
